theories/Nom_SyntaxBST.v
@@ -4,11 +4,12 @@ Set Implicit Arguments.
 Unset Strict Implicit.
 Unset Printing Implicit Defensive.
 Require Import Equations.Equations.
-From SendRec Require  Nom_Swap_fs.
+From SendRec Require Export  Nom_Swap_fs.
 Require Import Coq.ssr.ssreflect.
 Require Import Lia.
 Require Import PP.Ppsimplmathcomp.
 Require Import Equations.Equations.
+
 Require Import SendRec.Atom.
 
 
@@ -26,6 +27,8 @@ Inductive exp : Set :=
   | ff
   | var : atom -> exp
 .
+
+Locate atom.
 
 Definition exp_eqb e0 e1 : bool :=
 match (e0,e1) with
@@ -116,10 +119,7 @@ Fixpoint fv_exp (P : proc) : atoms :=
   | nu_ch nm P0 => (fv_exp P0)
 end.          
 
-Definition swap_aux (b c a : atom) := 
-  if (a == b) then c else if (a == c) then b else a.
 
-          
 Definition swap_exp (b c : atom) (e: exp)  : exp :=
   match e with
   | var nm => var (swap_aux b c nm)
@@ -137,6 +137,121 @@ Fixpoint swap (b c: atom) (P : proc) : proc :=
   | nu_ch nm P0 => nu_ch (swap_aux b c nm) (swap b c P0)
   end.
 
+
+(*
+Definition binder_eq_nm f (p0 p1 : (atom * proc)) : bool :=
+let (nm0,P0) := p0 in let (nm1,P1) := p1 in
+if (nm0 == nm1) then f P0 P1
+                               else if M.mem nm0 (fv_nm P1) then false 
+                               else f P0 (swap nm0 nm1 P1).
+
+
+Definition binder_eq_exp f (p0 p1 : (atom * proc)) : bool :=
+let (nm0,P0) := p0 in let (nm1,P1) := p1 in
+if (nm0 == nm1) then f P0 P1
+                               else if M.mem nm0 (fv_exp P1) then false 
+                               else f P0 (swap nm0 nm1 P1).
+
+*)
+
+Definition set_fresh (s :atoms) : atom := 
+  match atom_fresh s with
+  (exist x _) => x
+end. 
+(*
+Definition binder_eq_nm f (p0 p1 : (atom * proc)) : bool :=
+let (nm0,P0) := p0 in let (nm1,P1) := p1 in
+if (nm0 == nm1) then f P0 P1
+else let z := set_fresh (M.union (fv_nm P0) (fv_nm P1)) 
+      in f (swap nm0 z P0) (swap nm1 z P1).
+
+
+
+
+Definition binder_eq_exp f (p0 p1 : (atom * proc)) : bool :=
+let (nm0,P0) := p0 in let (nm1,P1) := p1 in
+if (nm0 == nm1) then f P0 P1
+else let z := set_fresh (M.union (fv_exp P0) (fv_exp P1)) 
+      in f (swap nm0 z P0) (swap nm1 z P1).*)
+
+Fixpoint proc_size (P : proc) : nat :=
+match P with
+| send _ _ P0 => 1 + (proc_size P0)
+| receive _ _ P0 => 1 + (proc_size P0)
+| throw _ _ P0 => 1 + (proc_size P0)
+| catch _ _ P0 => 1 + (proc_size P0)
+| par P0 P1 => 1 + (proc_size P0) + (proc_size P1)
+| inact => 1
+| nu_ch _ P0 => 1 + (proc_size P0)
+end.
+
+Lemma swap_size : forall a b P, proc_size (swap a b P) = proc_size P.
+Proof. 
+move=> a b P. elim P;
+do ? (move=> a0 e p H0/=//; rewrite H0//).
+rewrite e/=//. rewrite /=//.
+move => a0 p/= =>->//. 
+Qed.
+
+
+Obligation Tactic := move => *;do ? ((do ? rewrite swap_size); apply : leP; rewrite /=; ppsimpl;lia).
+(*
+Equations aeq (P0 P1 : proc) : bool by wf (proc_size P0)  :=
+aeq (send nm0 e0 P0') (send nm1 e1 P1') :=  (nm0 == nm1) && (e0 == e1) && (aeq P0' P1');
+aeq (receive nm0 nmb0 P0')  (receive nm1 nmb1 P1') :=  (nm0 == nm1) && if (nmb0 == nmb1) then aeq P0' P1' else aeq (swap nm0 (set_fresh (M.union (fv_exp P0') (fv_exp P1'))) P0') 
+                                                                                                               (swap nm1 (set_fresh (M.union (fv_exp P0') (fv_exp P1'))) P1');
+aeq (throw nm0 nm0' P0') (throw nm1 nm1' P1') := (nm0 == nm1) && (nm0' == nm1') && (aeq P0' P1');
+aeq (catch nm0 nmb0 P0') (catch nm1 nmb1 P1') := (nm0 == nm1) && if nmb0 == nmb1 then aeq P0' P1' else aeq (swap nm0 (set_fresh (M.union (fv_exp P0') (fv_exp P1'))) P0') 
+                                                                                                               (swap nm1 (set_fresh (M.union (fv_exp P0') (fv_exp P1'))) P1');
+aeq (nu_ch nm0 P0') (nu_ch nm1 P1') := if nm0 == nm1 then aeq P0' P1' else aeq (swap nm0 (set_fresh (M.union (fv_exp P0') (fv_exp P1'))) P0') 
+                                                                                                               (swap nm1 (set_fresh (M.union (fv_exp P0') (fv_exp P1'))) P1');
+aeq (par P0' P0'') (par P1' P1'') := (aeq P0' P1') && (aeq P0'' P1'');
+
+aeq inact inact := true;
+aeq _ _ := false.
+
+Fixpoint aeq_aux (n : nat) (P0 P1 : proc)  :=
+match n with 
+| 0 => false 
+| S n' => match P0, P1 with 
+         | (send nm0 e0 P0'),(send nm1 e1 P1') =>  (nm0 == nm1) && (e0 == e1) && (aeq_aux n' P0' P1')
+         | (receive nm0 nmb0 P0'), (receive nm1 nmb1 P1') => (nm0 == nm1) && if nmb0 == nmb1 then aeq_aux n' P0' P1' else aeq_aux n' (swap nm0 (set_fresh (M.union (fv_exp P0') (fv_exp P1'))) P0') 
+                                                                                                               (swap nm1 (set_fresh (M.union (fv_exp P0') (fv_exp P1'))) P1')
+         | (throw nm0 nm0' P0'), (throw nm1 nm1' P1') => (nm0 == nm1) && (nm0' == nm1') && (aeq_aux n' P0' P1')
+         | (catch nm0 nmb0 P0'), (catch nm1 nmb1 P1') => (nm0 == nm1) && if nmb0 == nmb1 then aeq_aux n' P0' P1' else aeq_aux n' (swap nm0 (set_fresh (M.union (fv_exp P0') (fv_exp P1'))) P0') 
+                                                                                                               (swap nm1 (set_fresh (M.union (fv_exp P0') (fv_exp P1'))) P1')
+         | (nu_ch nm0 P0'), (nu_ch nm1 P1') => if nm0 == nm1 then aeq_aux n' P0' P1' else aeq_aux n' (swap nm0 (set_fresh (M.union (fv_exp P0') (fv_exp P1'))) P0') 
+                                                                                                               (swap nm1 (set_fresh (M.union (fv_exp P0') (fv_exp P1'))) P1')
+         | (par P0' P0''),(par P1' P1'') => (aeq P0' P1') && (aeq P0'' P1'')
+
+         | inact, inact => true
+         |  _, _ => false
+         end
+end.
+
+Definition aeq2 p0 p1 := aeq_aux (proc_size p0) p0 p1.
+
+(*An alternative way to define functions whose termination is not immediate
+  I will try to experiment with this and the equations approach, to see which is nicest*)
+Lemma aeq2_size : forall p0 p1 n , aeq_aux (proc_size p0) p0 p1 = aeq_aux ((proc_size p0) + n) p0 p1.
+Proof. Admitted. *)
+
+(*
+Fixpoint aeq (P0 P1 : proc) {struct P0} : bool :=
+let binder_eq_nm := binder_eq_nm aeq in
+let binder_eq_exp := binder_eq_exp aeq in
+
+match P0,P1 with
+| (send nm0 e0 P0'), (send nm1 e1 P1') => (nm0 == nm1) && (e0 == e1) && (aeq P0' P1')
+| (receive nm0 nmb0 P0'), (receive nm1 nmb1 P1') => (nm0 == nm1) && (binder_eq_exp (nmb0, P0') (nmb1, P1'))
+| (throw nm0 nm0' P0'), (throw nm1 nm1' P1') => (nm0 == nm1) && (nm0' == nm1') && (aeq P0' P1')
+| (catch nm0 nmb0 P0'), (catch nm1 nmb1 P1') => (nm0 == nm1) && (binder_eq_nm (nmb0, P0') (nmb1, P1'))
+| (nu_ch nm0 P0), (nu_ch nm1 P1) => binder_eq_nm (nm0, P0) (nm1, P1)
+| (par P0' P0''),(par P1' P1'') => (aeq P0' P1') && (aeq P0'' P1'')
+| inact, inact => true
+| _, _ => false
+end.
+*)
 
 Definition binder_eq_nm f (p0 p1 : (atom * proc)) : bool :=
 let (nm0,P0) := p0 in let (nm1,P1) := p1 in
@@ -165,6 +280,8 @@ match P0,P1 with
 | inact, inact => true
 | _, _ => false
 end.
+
+
 
 Notation "P =A= Q" := (aeq P Q)(at level 70). 
 
@@ -202,6 +319,7 @@ Ltac gather_atoms ::=
 
 Definition alpha_variant (P : proc -> Prop) := forall p b c, P (swap_weak b c p) -> P p.
 
+(*
 Check proc_ind.
 Section PROC. 
 
@@ -234,7 +352,7 @@ Qed.
 
 End PROC.
 
-Check ind.
+Check ind.*)
 
 
 
@@ -244,33 +362,11 @@ Definition subst_exp (e : exp) (x : atom) (e_body : exp) : exp :=
   | t => t
   end.
 
-Fixpoint proc_size (P : proc) : nat :=
-match P with
-| send _ _ P0 => 1 + (proc_size P0)
-| receive _ _ P0 => 1 + (proc_size P0)
-| throw _ _ P0 => 1 + (proc_size P0)
-| catch _ _ P0 => 1 + (proc_size P0)
-| par P0 P1 => 1 + (proc_size P0) + (proc_size P1)
-| inact => 1
-| nu_ch _ P0 => 1 + (proc_size P0)
-end.
 
-Lemma swap_size : forall a b P, proc_size (swap a b P) = proc_size P.
-Proof. 
-move=> a b P. elim P;
-do ? (move=> a0 e p H0/=//; rewrite H0//).
-rewrite e/=//. rewrite /=//.
-move => a0 p/= =>->//. 
-Qed.
 
-Obligation Tactic := move => *;do ? ((do ? rewrite swap_size); apply : leP; rewrite /=; ppsimpl;lia).
 Check (fresh nil).
 Check (atom_fresh empty).  Check atom_fresh. 
 Check atom_fresh.
-Definition set_fresh (s :atoms) : atom := 
-  match atom_fresh s with
-  (exist x _) => x
-end. 
 
 
 Equations subst_proc_exp (e : exp) (x : atom) (P : proc) : proc by wf (proc_size P)  :=
@@ -296,11 +392,11 @@ subst_proc_nm a x (send nm e P0) := send (subst_nm a x nm) e (subst_proc_nm a x 
 subst_proc_nm a x (receive nm0 nm1 P0) := receive (subst_nm a x nm0) nm1 (subst_proc_nm a x P0);
 subst_proc_nm a x (throw nm0 nm1 P0) := throw (subst_nm a x nm0) (subst_nm a x nm1) (subst_proc_nm a x P0);
 subst_proc_nm a x (catch nm0 nm1 P0) := if x == nm1 then catch (subst_nm a x nm0) nm1 P0 
-                                                         else catch (subst_nm a x nm0) (set_fresh (add a (add x (fv_nm P0)))) (subst_proc_nm a x (swap nm1 (set_fresh (add a (add x (fv_nm P0)))) P0));
+                                                         else catch (subst_nm a x nm0) (set_fresh ((add a (add x(fv_nm (P0)))))) (subst_proc_nm a x (swap nm1 (set_fresh (add a (add x(fv_nm (P0))))) P0));
 subst_proc_nm a x (par P0 P1) := par (subst_proc_nm a x P0) ( subst_proc_nm a x P1);
 subst_proc_nm a x inact := inact;
 subst_proc_nm a x (nu_ch nm P0) := if x == nm then nu_ch nm P0 
-                                                   else nu_ch (set_fresh (add a (fv_nm P0))) (subst_proc_nm a x (swap nm (set_fresh (add a (fv_nm P0))) P0)).
+                                                   else nu_ch (set_fresh (add a (fv_nm (P0)))) (subst_proc_nm a x (swap nm (set_fresh (add a (add x (fv_nm (P0))))) P0)).
 
 Notation "nm{ x ::= a } t" := (subst_nm a x t) (at level 70).
 
@@ -322,62 +418,42 @@ Proof.
 move=> a0 a1. rewrite /predC1 /= Bool.negb_involutive. split; move/eqP=>->//=. 
 Qed.
 
+(*
 Lemma swap_aux_refl : forall a b, swap_aux a a b = b.
 Proof.
 move=> a b. rewrite /swap_aux. case : (eqVneq b a); done.
-Qed.
+Qed.*)
 
-Lemma swap_exp_refl : forall e a, swap_exp a a e = e.
+Lemma swap_exp_same : forall e a, swap_exp a a e = e.
 Proof.
 elim. 
 - move=> a. done. 
 - move=> a. done. 
-- move=> a a0. rewrite /swap_exp. rewrite swap_aux_refl. done. 
+- move=> a a0. rewrite /swap_exp. rewrite swap_aux_same.  done. 
 Qed.
 
-Lemma swap_refl : forall p a, swap a a p = p.
+Lemma swap_same : forall p a, swap a a p = p.
 Proof.
 elim.
-- move=> a e p IH a0. rewrite /swap -/swap swap_aux_refl. rewrite swap_exp_refl. f_equal. done. 
-- move=> a a0 p IH a1.  rewrite /swap -/swap swap_aux_refl. rewrite swap_aux_refl. f_equal. done. 
-- move=> a a0 p IH a1.  rewrite /swap -/swap swap_aux_refl. rewrite swap_aux_refl. f_equal. done.  
-- move=> a a0 p IH a1.  rewrite /swap -/swap swap_aux_refl. rewrite swap_aux_refl. f_equal. done.  
+- move=> a e p IH a0. rewrite /swap -/swap swap_aux_same. rewrite swap_exp_same. f_equal. done. 
+- move=> a a0 p IH a1.  rewrite /swap -/swap swap_aux_same. rewrite swap_aux_same. f_equal. done. 
+- move=> a a0 p IH a1.  rewrite /swap -/swap swap_aux_same. rewrite swap_aux_same. f_equal. done.  
+- move=> a a0 p IH a1.  rewrite /swap -/swap swap_aux_same. rewrite swap_aux_same. f_equal. done.  
 - move=> p IHp p0 IHp0 a.  rewrite /swap -/swap. rewrite IHp. rewrite IHp0. done. 
 - move => a. rewrite /=. done.
-- move=> a p IH a0.  rewrite /swap -/swap. rewrite IH. rewrite swap_aux_refl. done. 
+- move=> a p IH a0.  rewrite /swap -/swap. rewrite IH. rewrite swap_aux_same. done. 
 Qed.
 
 Ltac name_case a0 a1 := case : (eqVneq a0 a1).
 
-Lemma swap_inject : forall a a' bs bs', swap_aux bs bs' a = swap_aux bs bs' a' -> a  = a'.
-Proof.
-move => a a' bs bs'. rewrite /swap_aux.
-name_case a bs. 
-- move=>->. name_case a' bs.
- + move=>->. done.
- + name_case a' bs'. 
-  * move=>->. done.
-  * move=> /eqP H. move : (not_eq_sym H). done.
-- name_case a bs'.
- + move=>->.  name_case a' bs.
-  * move=>->. done.
-  * name_case a' bs'. 
-   ** move=>->. done.
-   ** move=> H1 H2 H3 H4. move : H4 H1 H2 H3=>->. move => _. move/eqP. done.
- + name_case a' bs.
-  * move=>->. move=> /eqP H _. done. 
-  * name_case a' bs'. 
-   ** move=>->. move => H1 H2 H3 H4. move : H4 H1 H2 H3=>->. move => _ _ /eqP. done.
-   ** done.
-Qed. 
 
-Definition swap_set bs bs' s := MapFunction.map (swap_aux bs bs') s. 
-
-
+(*
 Lemma in_swap_set : forall a bs bs' s, M.In a (swap_set bs bs' s) <-> exists a', M.In a' s /\ swap_aux bs bs' a' = a.
 Proof. 
 move => a bs bs' s. split;rewrite /swap_set; rewrite MapFunction.map_In //=; move=> x y-> //=.
 Qed.
+*)
+
 
 (*Some tactics*)
 Ltac contra := intros; subst; match goal with
@@ -401,6 +477,7 @@ Ltac if_destruct := (try rewrite eq_refl) ; match goal with
 Ltac if_destruct_r := repeat if_destruct.
 
 
+(*
 Lemma in_eqvt : forall a s bs bs', M.In a s <-> M.In (swap_aux bs bs' a) (swap_set bs bs' s).
 Proof. 
 move => a s bs bs'. split. 
@@ -412,9 +489,9 @@ move => a s bs bs'. split.
   **  if_destruct. if_destruct_r. 
   ** if_destruct_r. by move => + + + + <-.
 Qed.
+*)
 
-
-
+(*
 Lemma fv_nm_eqvt : forall P bs bs', M.Equal (swap_set bs bs' (fv_nm P)) (fv_nm (swap bs bs' P)).
 Proof. Admitted.
 
@@ -432,14 +509,42 @@ move => P a bs bs'. split. move => H2 H3. apply H2. rewrite in_eqvt.  rewrite fv
 Qed.
 
 Lemma swap_set_involutive : forall p bs bs', swap_set bs bs' (swap_set bs bs' p) = p.
-Proof. Admitted.
+Proof. Admitted.*)
+
+Lemma swap_fs_singleton : forall a bs bs', swap_fs bs bs' (singleton a) [=] singleton (swap_aux bs bs' a).
+Proof.
+move => a bs bs'. rewrite /swap_fs !singleton_b. Print MF. rewrite /eqb. simpl_swap_aux. done. fsetdec.  fsetdec. fsetdec. 
+Qed.
+
+Lemma fv_nm_eqvt : forall P bs bs', (fv_nm (swap bs bs' P)) [=] (swap_fs bs bs' (fv_nm P)).
+Proof. 
+elim; try solve [intros; rewrite /=; (do ? rewrite -union_swap_fs); rewrite H; rewrite !swap_fs_singleton;  done].
+- intros. rewrite /=.
+  rewrite -union_swap_fs. rewrite H. rewrite swap_fs_singleton. rewrite -remove_swap_fs. fsetdec. 
+- intros. rewrite /=.
+  rewrite -union_swap_fs. rewrite H H0. done. 
+- move => bs bs'. rewrite /=. fsetdec. 
+- intros. rewrite /=. rewrite -remove_swap_fs. rewrite H. done.
+Qed.
 
 
 Ltac forget_tac IH :=  
-  rewrite /fv_nm -/fv_nm; simp subst_proc_nm;
+(*  move => a b; *)rewrite /fv_nm -/fv_nm; simp subst_proc_nm;
   rewrite /subst_nm; if_destruct; (try fsetdec);
-  let H := fresh "H__in" in move=> H; rewrite /= ?eq_refl /=; apply IH; fsetdec.
+  let H := fresh "H__in" in move=> H; simp aeq; rewrite /= ?eq_refl /=; apply IH; fsetdec.
 
+(*
+Lemma aeq_refl : forall P , P =A= P.
+Proof. 
+elim.
+- move => k e p H. simp aeq. by rewrite /= 2!eq_refl. 
+- move => k ep H. simp aeq. rewrite !eqxx. done . 
+- move => k e p H. simp aeq. rewrite !eqxx. done. 
+- move => k k' p H. simp aeq. rewrite !eqxx. done. 
+- move => k k' p H.  simp aeq. rewrite /= ?eq_refl. apply/andP. split; done.  
+- rewrite /=. done. 
+- move => k p H. simp aeq. by rewrite /= ?eq_refl. 
+Qed.*)
 Lemma aeq_refl : forall P , P =A= P.
 Proof. 
 elim.
@@ -451,6 +556,8 @@ elim.
 - rewrite /=. done. 
 - move => k p H. by rewrite /= ?eq_refl. 
 Qed.
+
+
 
 
 
@@ -480,23 +587,59 @@ move => a b. rewrite /subst_nm. rewrite eq_refl. done.
 Qed. 
 
 
-
-Check ind.
-(*This lemma is used in forget*)
-Lemma subst_fresh : forall p a b x x0, ~ M.In x (M.union (singleton a) (singleton b)) -> 
-                                  ~ M.In x0 (M.union (singleton a) (singleton b)) -> swap x x0 (p{ a ::= b } p) = (p{ a ::= b} swap x x0 p).
-Proof. Admitted.
+(*Don't prove this lemma, it won't be needed later*)
 Lemma swap_aeq : forall p p' bs bs', p =A= p' -> swap bs bs' p =A= swap bs bs' p'.
 Proof. Admitted.
 
+Lemma swap_exp_comm : forall p bs bs', swap_exp bs bs' p = swap_exp bs' bs p.
+Proof. move => p bs bs'. rewrite /swap_exp. destruct p. done. done. simpl_swap_aux. 
+Qed.
+
+(*A variantion of  this lemma will be needed later*)
 Lemma swap_comm : forall p bs bs', swap bs bs' p = swap bs' bs p.
 Proof. Admitted.
+
+
 Require Import Wellfounded. 
 Check (well_founded_induction
                      (wf_inverse_image _ nat _ (@proc_size)
                         PeanoNat.Nat.lt_wf_0)).
 
 (*By size induction*)
+
+Lemma subst_eqvt : forall P a b bs bs',  swap bs bs' (p{a::= b} P) =A= p{ (swap_aux bs bs' a) ::= (swap_aux bs bs' b)} swap bs bs' P.
+Proof. Admitted.
+
+Lemma aeq_trans : forall P0 P1 P2, P0 =A= P1 -> P1 =A= P2 -> P0 =A= P2.
+Proof. Admitted.
+
+Lemma swap_involutive : forall P bs bs', swap bs bs' (swap bs bs' P) = P.
+Proof. Admitted.
+
+Lemma swap_exp_eqvt : forall e bs0 bs1 bs2 bs3, swap_exp bs0 bs1 (swap_exp bs2 bs3 e) = swap_exp (swap_aux bs0 bs1 bs2) (swap_aux bs0 bs1 bs3) (swap_exp bs0 bs1 e).
+Proof.
+intros. rewrite /swap_exp. destruct e. done. done. f_equal. apply swap_aux_equivariance. 
+Qed.
+
+
+
+Lemma swap_eqvt : forall P bs0 bs1 bs2 bs3, swap bs0 bs1 (swap bs2 bs3 P) = swap (swap_aux bs0 bs1 bs2) (swap_aux bs0 bs1 bs3) (swap bs0 bs1 P).
+Proof. Locate lt_wf. Check  Wf_nat.lt_wf.
+induction P using (well_founded_induction
+                     (wf_inverse_image _ nat _ (@proc_size)
+                       Wf_nat.lt_wf )).
+move => bs0 bs1 bs2 bs3.
+destruct P.
+- rewrite /swap -/swap. f_equal. apply swap_aux_equivariance. apply swap_exp_eqvt. apply H. done. 
+- rewrite /swap -/swap. f_equal. all : try apply swap_aux_equivariance.  apply H. done. 
+- rewrite /swap -/swap. f_equal. all : try apply swap_aux_equivariance.  apply H. done. 
+- rewrite /swap -/swap. f_equal. all : try apply swap_aux_equivariance.  apply H.  done. 
+- rewrite /swap -/swap. f_equal. apply H. auto. apply / leP. rewrite /=.  ppsimpl. lia.  
+  apply H. auto. apply / leP. rewrite /=.  ppsimpl. lia.  
+- rewrite /swap -/swap. done. 
+- rewrite /swap -/swap. f_equal. apply swap_aux_equivariance. apply H. done. 
+Qed.
+
 Lemma forget : forall  P a b, ~ M.In a (fv_nm P) ->  (p{a::= b} P) =A= P.
 Proof.
 move => + a b. induction P using (well_founded_induction
@@ -518,57 +661,80 @@ destruct P.
    ** fsetdec. 
    **  move => H2 H3. rewrite /aeq -/aeq eq_refl /=. 
        rewrite /set_fresh. destruct (atom_fresh ((add b (add a(fv_nm P))))). if_destruct. 
-    *** rewrite swap_refl. move => H5. apply H.  auto. move : H5=> /eqP => H4. have H__in: ~ M.In t0 ((singleton a)).  fsetdec. fsetdec. 
+    *** rewrite swap_same. move => H5. apply H.  auto. move : H5=> /eqP => H4. have H__in: ~ M.In t0 ((singleton a)).  fsetdec. fsetdec. 
     *** have: M.mem x (fv_nm P) = false. rewrite <- F.not_mem_iff. fsetdec. move=>->. move => H4 H5. rewrite swap_comm. 
         apply H;auto. 
      **** rewrite swap_size. auto.
-     **** rewrite -fv_nm_eqvt. rewrite (in_eqvt _ _ x t0). rewrite swap_set_involutive. rewrite /swap_aux. move : n.  if_destruct.
-      ***** fsetdec. 
-      ***** if_destruct. move : i0=> /eqP => H5. have : ~ M.In a (singleton t0) by fsetdec. fsetdec.
+     **** rewrite fv_nm_eqvt. apply swap_fs_4. simpl_swap_aux; fsetdec. 
 Admitted.
 
 Lemma forget : forall  P a b, ~ M.In a (fv_nm P) ->  (p{a::= b} P) =A= P.
 Proof.
-move => + a b. apply  (@ind (M.union (M.singleton a) (M.singleton b)) (fun P => ~ M.In a (fv_nm P) -> (p{ a ::= b} P) =A= P)). 
-- admit. 
-- move => t e p IH. forget_tac IH. 
-- move => k x p H__nin IH. forget_tac IH.
-- move => k x p IH. 
-  rewrite /fv_nm -/fv_nm; simp subst_proc_nm. Print exp.
+induction P using (well_founded_induction
+                     (wf_inverse_image _ nat _ (@proc_size)
+                        PeanoNat.Nat.lt_wf_0)).
+destruct P. 
+-  forget_tac H. 
+-  forget_tac H. 
+-  move => a b. rewrite /fv_nm -/fv_nm; simp subst_proc_nm. Print exp.
   rewrite /subst_nm.  if_destruct_r; (try fsetdec).
-  move => neq H__in. rewrite /= ?eq_refl /=. apply IH. fsetdec. 
-- move => k x p _ IH. rewrite /fv_nm -/fv_nm. 
+  move => neq H__in. simp aeq; rewrite /= ?eq_refl /=. apply H. fsetdec. fsetdec. 
+- move => a b.  rewrite /fv_nm -/fv_nm. 
   simp  subst_proc_nm.  
   if_destruct. 
   * rewrite /subst_nm. if_destruct. 
-   ** move => H2. fsetdec. 
-   ** rewrite aeq_refl. done. 
+   ** fsetdec. 
+   ** by rewrite aeq_refl. 
   * rewrite /subst_nm. if_destruct. 
    ** fsetdec. 
-   **  move => H2 H3. rewrite /aeq -/aeq eq_refl /=. 
-       rewrite /set_fresh. destruct (atom_fresh ((add b (add a(fv_nm p))))). name_case x0 x. 
-    *** move=>->.   rewrite swap_refl. apply IH.  move : H2=> /eqP => H4. have H__in: ~ M.In x ((singleton a)).  fsetdec. fsetdec. 
-    *** have: M.mem x0 (fv_nm p) = false. rewrite <- F.not_mem_iff. fsetdec. move=>->.
-  
-      apply singleton_iff.        Locate "!=". fsetdec.
-        if_destruct.
-    *** rewrite swap_refl. move => H5. apply IH. fsetdec. (*freshness of x is needed here*)
-    *** have: M.mem x0 (fv_nm p) = false. rewrite <- F.not_mem_iff. fsetdec. 
-        move =>->. move => H H2. rewrite swap_comm. rewrite -subst_fresh.  
-     **** apply swap_aeq. apply IH. fsetdec. 
-     **** fsetdec. 
-     **** fsetdec.      
+   **  move => H2 H3. simp aeq. rewrite eq_refl /=. 
+       rewrite /set_fresh. destruct ( atom_fresh (add b (add a(fv_nm P)))). if_destruct.
+    *** rewrite swap_same. move => H5. apply H.  auto. move : H5=> /eqP => H4. fsetdec. 
+    ***(* have: M.mem x (fv_nm P) = false. rewrite <- F.not_mem_iff. fsetdec. move=>->.*) move => H4 H5. destruct (atom_fresh (fv_exp (p{ a ::= b} swap t0 x P) `union` fv_exp P)). 
+         apply: aeq_trans. apply : subst_eqvt. rewrite swap_eqvt. simpl_swap_aux; try fsetdec. 
+     **** auto. apply H. auto. 
+     **** rewrite swap_size. auto.
+     **** rewrite fv_nm_eqvt. apply swap_fs_4. simpl_swap_aux. (*Need stronger freshness assumption for generated variable here*) fsetdec. fsetdec. fsetdec. 
+Admitted.
+
+
+
+Lemma renaming : forall P a b c, ~ M.In c (fv_nm P) -> p{ c ::= b} (swap c a P) =A= p{ a ::= b} P.
+Proof.
+move => + a b. induction P using (well_founded_induction
+                     (wf_inverse_image _ nat _ (@proc_size)
+                        PeanoNat.Nat.lt_wf_0)).
+destruct P.
 - admit. 
 - admit.
--admit. 
+- admit. 
+rewrite /swap -/swap /fv_nm -/fv_nm. simpl_swap_aux; try fsetdec. 
+ * simp subst_proc_nm. move : C.  if_destruct. if_destruct. move => H1 H2 H3. rewrite /set_fresh. 
+    destruct (atom_fresh (add b (add c (fv_nm (swap c a P))))). 
+    destruct (atom_fresh (add b (add a (fv_nm P)))). rewrite /=. if_destruct. 
+  ** rewrite /subst_nm !eqxx. move => _. rewrite /=. rewrite swap_eqvt. simpl_swap_aux.
+   *** rewrite swap_involutive swap_same. rewrite /=. apply aeq_refl.
+Set Printing All. if_destruct. rewrite (eq_sym a c). if_destruct. if_destruct. move => _ + H. rewrite /set_fresh.
+    destruct (atom_fresh (add b (add c (fv_nm (swap c a P))))). 
+    destruct (atom_fresh (add b (add a (fv_nm P)))). rewrite /subst_nm !eqxx.
+    rewrite /aeq -/aeq eqxx /=. move : n n0. if_destruct. 
+   *** rewrite swap_swap /swap_aux. if_destruct. if_destruct. fsetdec. rewrite swap_swap. rewrite /swap_aux. if_destruct. if_destruct. fsetdec.  if_destruct. move => H1 H2 H3 H4 H5 H6 H7 H8 H9 H10. rewrite swap_comm. aplpy H. rewrite swap_size. auto. rewrite -fv_nm_eqvt. 
+  rewrite (in_eqvt _ _ c x0). rewrite swap_set_involutive. rewrite /swap_aux eqxx. fsetdec. 
+   *** move => H1 H2 H3 H4 H5 H6. have: M.mem x (fv_nm P) = false. rewrite <- F.not_mem_iff. have: ~M.In x (fv_nm (swap c a P)). fsetdec. rewrite -fv_nm_eqvt. rewrite (in_eqvt _ _ c a). rewrite swap_set_involutive. rewrite /swap_aux. move : H3. if_destruct. fsetdec. move : H4. if_destruct. fsetdec. move=>->. move => H4 H5. rewrite swap_comm. 
+        apply H;auto. 
+
+move : n. if_destruct. (*Need stronger freshness assumption for generated variable here*)fsetdec. 
+          if_destruct. move : i0=> /eqP => H5. fsetdec. 
 Admitted.
+
+rewrmove/eq_sym.
 
 Ltac forget_tac2 IH :=  
   rewrite /fv_nm -/fv_nm; simp subst_proc_nm;
   rewrite /subst_nm; if_destruct; (try fsetdec);
   let H := fresh "H__in" in move=> H; rewrite /= ?eq_refl /=; move=>H2; apply H; fsetdec.
 
-Lemma forget2 : forall  P a b, ~ M.In a (fv_nm P) ->  (p{a::= b} P) =A= P.
+Lemma forget3 : forall  P a b, ~ M.In a (fv_nm P) ->  (p{a::= b} P) =A= P.
 Proof.
 move => P a b. funelim  (p{ a ::= b} P).
 -  rewrite /fv_nm -/fv_nm; simp subst_proc_nm.
@@ -583,16 +749,17 @@ move => P a b. funelim  (p{ a ::= b} P).
   rewrite /subst_nm.  if_destruct_r; (try fsetdec).
   move => neq H__in. rewrite /= ?eq_refl /=. move => H2. apply H. fsetdec. 
 - rewrite /fv_nm -/fv_nm. 
-  simp  subst_proc_nm.  
+  simp  subst_proc_nm. move : Heqcall.  
   if_destruct. 
   * rewrite /subst_nm. if_destruct. 
    ** move => H2. fsetdec. 
    ** rewrite aeq_refl. done. 
   * rewrite /subst_nm. if_destruct. 
    ** fsetdec. 
-   **  move => H2 H3 H4. rewrite /aeq -/aeq eq_refl /=. 
-    *** rewrite /set_fresh.  destruct (atom_fresh (add a (add x (fv_nm p2)))). 
-        if_destruct.  
+   **  move => H2 H3. (* rewrite /aeq -/aeq eq_refl -/fv_nm /= -/fv_nm.  *)
+    *** move : H. rewrite /set_fresh.  destruct (atom_fresh (add a (add x (fv_nm p2)))). move=> H H4 H5.   apply H. move => + ->.  
+        simp subst_proc_nm. move : H3. if_destruct.  rewrite /subst_nm. move : H2. if_destruct. rewrite /set_fresh.
+        destruct (atom_fresh (add a (add x (fv_nm p2)))).
     *** rewrite swap_refl. move => H5. apply H. fsetdec. 
     ***  rewrite /set_fresh. destruct (atom_fresh ((add b (add a(fv_nm p))))). have: M.mem x0 (fv_nm p) = false. rewrite <- F.not_mem_iff. fsetdec. move =>->. move => H H2.
          rewrite -subst_fresh.  
